hoare

coq/Hoare.v
@@ -3,47 +3,839 @@ Require Import Unicode.Utf8.
 
 Require Import Koika.TypedSyntax.
 Require Import Koika.TypedSemantics.
+Require Import Koika.TypedParsing.
+
+Require Import Koika.SemanticProperties.
+(* for more details about hoare triples refer to the
+ * software foundations book:
+ * https://softwarefoundations.cis.upenn.edu/plf-current/Hoare.html
+ *)
+
+
+Lemma log_find_empty : ∀ reg_t {R : reg_t -> type} {REnv : Env reg_t} T r fn ,
+  @log_find _ R REnv T log_empty r fn = None.
+Proof.
+  intros. unfold log_empty, log_find. now rewrite getenv_create.
+Qed.
+
+Lemma log_app_empty_l : ∀ reg_t {R : reg_t -> type} {REnv : Env reg_t} (l : Log R REnv),
+  log_app log_empty l = l.
+Proof.
+  intros. apply equiv_eq.
+  unfold equiv, log_app, map2, log_empty. intro.
+  rewrite ?getenv_create.
+  apply List.app_nil_l.
+Qed.
+
+Lemma log_app_empty_r : ∀ reg_t {R : reg_t -> type} {REnv : Env reg_t} (l : Log R REnv),
+  log_app l log_empty = l.
+Proof.
+  intros. apply equiv_eq.
+  unfold equiv, log_app, map2, log_empty. intro.
+  rewrite ?getenv_create.
+  apply List.app_nil_r.
+Qed.
+
+Lemma latest_write_cons_read : ∀ reg_t `{FiniteType reg_t} {R : reg_t -> type} {REnv : Env reg_t} (l : Log R REnv) r1 r2 p,
+  latest_write (log_cons r1 {| kind := LogRead; port := p; val := tt |} l) r2 = latest_write l r2.
+Proof.
+  intros; unfold latest_write, log_find, log_cons.
+  destruct (eq_dec r1 r2) as [Heq|Hneq].
+  + now rewrite Heq, get_put_eq.
+  + now rewrite get_put_neq.
+Qed.
+
+Lemma commit_read : ∀ reg_t `{FiniteType reg_t} {R : reg_t -> type} {REnv : Env reg_t} (l : Log R REnv) reg port env,
+  commit_update env (log_cons reg {| kind := LogRead; port := port; val := tt |} l) = commit_update env l.
+Proof.
+  intros; unfold commit_update.
+  apply create_funext; intro.
+  now rewrite latest_write_cons_read.
+Qed.
+
+Lemma commit_read_log : ∀ reg_t {R : reg_t -> type} {REnv : Env reg_t} (l : Log R REnv) env,
+  (∀ reg, log_existsb l reg is_write0 = false) ->
+  (∀ reg, log_existsb l reg is_write1 = false) ->
+  commit_update env l = env.
+Proof.
+  intros; unfold commit_update.
+  apply equiv_eq; intro.
+  rewrite getenv_create.
+  now rewrite latest_write_None.
+Qed.
+
+Lemma list_find_opt_app_some : ∀ A B l l' x (fn: A -> option B),
+  list_find_opt fn l = Some x -> list_find_opt fn (l ++ l') = Some x.
+Proof.
+  intros.
+  induction l. inversion H.
+  cbn in H.
+  destruct (fn a) eqn:Ha.
+  cbn. now rewrite Ha, H.
+  cbn. rewrite Ha.
+  auto.
+Qed.
+
+Lemma list_find_opt_app_none : ∀ A B l l' (fn: A -> option B),
+  list_find_opt fn l = None -> list_find_opt fn (l ++ l') = list_find_opt fn l'.
+Proof.
+  intros.
+  induction l. reflexivity.
+  cbn in H.
+  destruct (fn a) eqn:Ha.
+  inversion H.
+  cbn. rewrite Ha.
+  auto.
+Qed.
+
+Lemma commit_update_app : ∀ reg_t(*  `{FiniteType reg_t}  *){R : reg_t -> type} {REnv : Env reg_t} (l1 l2 : Log R REnv) env,
+  commit_update (commit_update env l2) l1 = commit_update env (log_app l1 l2).
+Proof.
+  intros.
+  unfold commit_update.
+  apply create_funext.
+  intro.
+  rewrite getenv_create.
+  destruct (latest_write l1 k) eqn:Hl2.
+  unfold log_app, map2.
+  unfold latest_write, log_find.
+  rewrite getenv_create.
+  erewrite list_find_opt_app_some. reflexivity. assumption.
+  unfold latest_write, log_find, log_app, map2. rewrite getenv_create. now rewrite list_find_opt_app_none.
+Qed.
+
+(* Lemma log_cons_empty : ∀ reg_t {R : reg_t -> type} {REnv : Env reg_t} le,
+  @log_cons _ R REnv reg el log_empty = . *)
+
+Lemma log_app_inv_tail : ∀ reg_t {R : reg_t -> type} {REnv : Env reg_t} (l l1 l2: Log R REnv),
+ log_app l1 l = log_app l2 l ->
+ l1 = l2.
+Proof.
+  intros reg_t R REnv * H.
+  apply equiv_eq in H.
+  unfold log_app, equiv in H.
+  setoid_rewrite getenv_map2 in H.
+  setoid_rewrite app_inv_tail_iff in H.
+  apply equiv_eq in H.
+  assumption.
+Qed.
+
+Lemma may_read_empty : ∀ reg_t {R : reg_t -> type} {REnv : Env reg_t} p r,
+  @may_read _ R REnv log_empty log_empty p r = true.
+Proof.
+  intros.
+  unfold may_read.
+  destruct p; [apply andb_true_iff; split|];
+  now rewrite log_existsb_app, negb_true_iff, log_existsb_empty.
+Qed.
+
+Lemma log_cons_app : ∀ reg_t {R : reg_t -> type} {REnv : Env reg_t} r le (l1 l2: Log R REnv),
+  log_cons r le (log_app l1 l2) = log_app (log_cons r le l1) l2.
+Proof.
+  intros.
+  unfold log_cons.
+  apply equiv_eq.
+  unfold equiv.
+  intros.
+  unfold log_cons, log_app, map2, equiv.
+  intro.
+  (* unfold log_cons, log_app, map2. *)
+  (* assert (getenv REnv (create REnv (λ k : reg_t, getenv REnv l1 k ++ getenv REnv l2 k)) r =
+          getenv REnv ()) *)
+
+  (* , equiv. *)
+  (* intro. *)
+  rewrite ?getenv_create.
+  rewrite app_comm_cons.
+Admitted.
 
 Section Hoare.
 
-  Context {pos_t var_t fn_name_t reg_t ext_fn_t: Type}.
+  Context {pos_t (* var_t *) fn_name_t reg_t ext_fn_t: Type}.
   Context {R: reg_t -> type}.
   Context {Sigma: ext_fn_t -> ExternalSignature}.
 
-  Notation action := (action pos_t var_t fn_name_t R Sigma).
+  (* Notation action := (action pos_t var_t fn_name_t R Sigma). *)
 
   (* Register environment a Map-Type from register names to their values *)
   Context {REnv: Env reg_t}.
 
-  Context {sig: tsig var_t}.
+  (** An _assertion_ is a logical claim about the state of a circuit
 
-  Definition assertion := tcontext sig -> Log R REnv -> REnv.(env_t) R -> Prop.
+    This state consists of the register environment, the variable valuation (Gamma/Γ),
+    the scheduler log and the current action log.
 
-  Inductive HoareTriple {tau: type} : assertion -> action sig tau -> assertion -> Prop :=
-  | HTSeq : ∀ P Q R a1 a2,
-    HoareTriple P a1 Q -> HoareTriple Q a2 R ->
-    HoareTriple P (Seq a1 a2) R.
+    Unfortunately, the scheduler/action log and the register environment cannot be
+    combined into a single 'register state'. One might think it should be possible,
+    since problems like multiple writes to the same register are already eliminated
+    by assuming (in `hoare_triple`) that `interp_action` evaluated to `Some _`. However,
+    consider the case where a read0 is used after a write0 (which is considered ugly but
+    legal koika). In this case the read0 should observe the value from the beginning of
+    the cycle. However when merging the logs and the environment into a single state - we
+    would no longer know if the register value in this state is still the one from the
+    beginning of the cycle or the one from a previous `write1`.
 
-  Declare Scope log_scope.
-  Notation "[]" := log_empty : log_scope.
-  Bind Scope log_scope with Log.
+    Letz go over that again with a specific example. Assume we would have merge the
+    logs and the env. Now we would like to proov this property.
 
-  Definition interp_action_update_env {tau} env sigma Gamma slog alog (act : action sig tau) :=
-    option_map (fun '(l, r, Gamma') => (commit_update env l, r, Gamma')) (interp_action (REnv := REnv) env sigma Gamma slog alog act).
+    {{ reg = 5 }} <{ read0(reg) }> {{ ret = 5 }}
 
-  Theorem hoare_triple_interp_action {tau} : ∀ P (a : action sig tau) Q,
-    HoareTriple P a Q ->
-    ∀ env log Γ Γ' sigma r slog alog,
-    P Γ alog env ->
-    interp_action env sigma Γ slog alog a = Some (log, r, Γ') ->
-    Q Γ' log env.
+    However, we would fail, as coq would bring to our attention that `reg = 5` might also
+    be the result of `env[reg] = 3` and `actionlog = [write0(reg, 5)]`.
+
+    So its turns out, we actually cannot prove our postcondition in every possible state that
+    satisfies our precondition.
+    *)
+
+  Lemma log_app_assoc : ∀ reg_t {R : reg_t -> type} {REnv : Env reg_t} (l1 l2 l3 : Log R REnv),
+    log_app l1 (log_app l2 l3)  = log_app (log_app l1 l2) l3.
   Proof.
-    induction 1.
+    intros.
+    unfold log_app, map2. apply equiv_eq. unfold equiv. intro.
+    rewrite ?getenv_create.
+    apply List.app_assoc.
+  Qed.
+
+  Lemma commit_update_empty : ∀ (env : REnv.(env_t) R),
+    commit_update env log_empty = env.
+  Proof.
+    intros.
+    unfold commit_update.
+    apply equiv_eq.
+    unfold equiv.
+    intros.
+    rewrite getenv_create.
+    unfold latest_write. now rewrite log_find_empty.
+  Qed.
+
+  Local Ltac simple_interp_some :=
+    repeat match goal with
+    | H: interp_action _ _ _ _ _ ?a = Some _ |- _ => head_constructor a; simpl in H
+    | H: opt_bind ?a _ = Some _ |- _ => destruct a eqn:?Heq; inversion H; clear H
+    | H: prod _ _ |- _ => destruct H
+    | H: and _ _ |- _ => destruct H
+    | H: Some _ = Some _ |- _ => apply Some_inj in H
+    | H: pair _ _ = pair _ _ |- _ => apply pair_inj in H
+    | _ => progress subst
+    end.
+
+  Ltac solve_log_irrelevance :=
+    repeat match goal with
+    | H: ∀ _ _ _ _ _ _ _ _ _ _ _ _ _ _ _,
+      interp_action _ _ _ _ (log_app _ _) _ = Some _ ->
+      interp_action _ _ _ (log_app _ _) _ _ = Some _ -> _,
+      H1: interp_action _ _ _ ?l1 (log_app ?l2 ?l3) ?a = Some _,
+      H2: interp_action _ _ _ (log_app ?l3 ?l1) ?l2 ?a = Some _ |- _ =>
+      pose_once (H _ _ a _ _ _ _ _ _ _ _ _ _ _ _ H1 H2)
+    | H: log_app _ ?l = log_app _ (log_app _ ?l) |- _ =>
+      rewrite log_app_assoc in H;
+      apply log_app_inv_tail in H
+    | H: (if ?cond then Some _ else None) = Some _ |- _ =>
+    destruct (cond) eqn:?Hc; inversion H
+    | _ => progress simple_interp_some
+    end;
+    try solve [repeat match goal with
+    | |- and _ _ => split
+    | |- log_app (log_app _ _) _ = log_app _ (log_app _ _) => apply eq_sym, log_app_assoc
+    | |- _ => solve [assumption + reflexivity + discriminate]
+    end].
+
+  Section Args.
+(*
+  Fixpoint interp_log_irrelevance' sig tau (a : action' R Sigma (sig := sig) (tau := tau)): ∀ (env : REnv.(env_t) R) sigma Γ Γ' Γ'' slog alog alog' alog_out alog_out'  r r',
+    interp_action env sigma Γ slog (log_app alog' alog) a = Some (alog_out, r, Γ') ->
+    interp_action env sigma Γ (log_app alog slog) alog' a = Some (alog_out', r', Γ'') ->
+
+    (log_app alog_out slog) = (log_app alog_out' (log_app alog slog)) /\ r = r' /\ Γ' = Γ''.
+    Context (interp_action:
+                forall {sig: tsig var_t} {tau}
+                  (Gamma: tcontext sig)
+                  (sched_log: Log) (action_log: Log)
+                  (a: action sig tau),
+                  option (Log * type_denote tau * (tcontext sig))).
+
+    Fixpoint interp_args'
+              {sig: tsig var_t}
+              (Gamma: tcontext sig)
+              (sched_log: Log)
+              (action_log: Log)
+              {argspec: tsig var_t}
+              (args: acontext sig argspec)
+      : option (Log * tcontext argspec * (tcontext sig)) :=
+      match args with
+      | CtxEmpty => Some (action_log, CtxEmpty, Gamma)
+      | @CtxCons _ _ argspec k_tau arg args =>
+        let/opt3 action_log, ctx, Gamma := interp_args' Gamma sched_log action_log args in
+        let/opt3 action_log, v, Gamma := interp_action _ _ Gamma sched_log action_log arg in
+        Some (action_log, CtxCons k_tau v ctx, Gamma)
+      end.
+  End Args. *)
+  Fixpoint interp_log_irrelevance' sig tau (a : action' R Sigma (sig := sig) (tau := tau)): ∀ (env : REnv.(env_t) R) sigma Γ Γ' Γ'' slog alog alog' alog_out alog_out'  r r',
+    interp_action env sigma Γ slog (log_app alog' alog) a = Some (alog_out, r, Γ') ->
+    interp_action env sigma Γ (log_app alog slog) alog' a = Some (alog_out', r', Γ'') ->
+
+    (log_app alog_out slog) = (log_app alog_out' (log_app alog slog)) /\ r = r' /\ Γ' = Γ''.
+    (* one should be able to show that r = r' and Γ' = Γ'' *)
+  Proof.
+    destruct a; cbn; intros.
+    - discriminate.
+    - inversion H; inversion H0. subst. repeat split. auto using log_app_assoc.
+    - inversion H; inversion H0. subst. repeat split. auto using log_app_assoc.
+    - solve_log_irrelevance.
+    - solve_log_irrelevance.
+    - solve_log_irrelevance.
+    - solve_log_irrelevance.
+      destruct (Bits.single t0);
+      solve_log_irrelevance.
+    - solve_log_irrelevance.
+      repeat split.
+      now rewrite log_app_assoc, log_cons_app.
+      now rewrite log_app_assoc.
+    - solve_log_irrelevance.
+      repeat split.
+      now rewrite log_app_assoc, log_cons_app.
+    - solve_log_irrelevance.
+    - solve_log_irrelevance.
+    - solve_log_irrelevance.
+    - solve_log_irrelevance.
+      enough (∀ alo alo' r r' Γ Γ' Γ'',
+        interp_args env sigma Γ slog (log_app alog' alog) args = Some (alo, r, Γ') ->
+        interp_args env sigma Γ (log_app alog slog) alog' args = Some (alo', r', Γ'') ->
+        (log_app alo slog) = (log_app alo' (log_app alog slog)) /\ r = r' /\ Γ' = Γ''
+      ).
+      + specialize (H _ _ _ _ _ _ _ Heq0 Heq).
+        solve_log_irrelevance.
+      + clear Heq Heq0 Heq1 Heq2 fn t0 t1 t4 t5 l l1 r r'.
+        induction args.
+        * intros. cbn in H, H0.
+          solve_log_irrelevance.
+        * intros. cbn in H, H0.
+          solve_log_irrelevance.
+          specialize (IHargs _ _ _ _ _ _ _ Heq0 Heq).
+          solve_log_irrelevance.
+    - solve_log_irrelevance.
+  Qed.
+
+  Lemma interp_log_irrelevance sig tau (a : action' R Sigma (sig := sig) (tau := tau)) :
+    ∀ (env : REnv.(env_t) R) sigma Γ Γ' Γ'' slog alog alog_out alog_out'  r r',
+    interp_action env sigma Γ slog alog a = Some (alog_out, r, Γ') ->
+    interp_action env sigma Γ (log_app alog slog) log_empty a = Some (alog_out', r', Γ'') ->
+
+    (log_app alog_out slog) = log_app alog_out' (log_app alog slog).
+  Proof.
+    intros.
+    rewrite <- (log_app_empty_l _ alog) in H.
+    pose proof (interp_log_irrelevance' _ _ _ _ _ _ _ _ _ _ _ _ _ _ _ H H0).
+    destruct H1.
+    auto.
+  Qed.
+
+
+  Ltac solve_log_irrelevance' :=
+    repeat match goal with
+    | H: ∀ _ _ _ _ _ _ _ _ _ _ _ _ _ _ _,
+      interp_action _ _ _ (log_app _ _) _ _ = Some _ ->
+      interp_action _ _ _ _ _ _ = Some _ -> _,
+      H1: interp_action ?env _ _ (log_app ?l1 ?l2) _ ?a = Some _,
+      H2: interp_action (commit_update ?env ?l2) _ _ ?l1 _ ?a = Some _ |- _ =>
+      pose_once (H _ _ _ _ _ _ _ _ _ _ _ _ _ _ _ H1 H2)
+    | H: log_app _ ?l = log_app _ (log_app _ ?l) |- _ =>
+      rewrite log_app_assoc in H;
+      apply log_app_inv_tail in H
+    | H: (if ?cond then Some _ else None) = Some _ |- _ =>
+    destruct (cond) eqn:?Hc; inversion H
+    | _ => progress simple_interp_some
+    end;
+    try solve [repeat match goal with
+    | |- and _ _ => split
+    | |- log_app (log_app _ _) _ = log_app _ (log_app _ _) => apply eq_sym, log_app_assoc
+    | |- _ => solve [assumption + reflexivity + discriminate]
+    end].
+
+  Lemma option_match_eq : ∀ A (o o' : option A) d,
+  match
+    match o with
+    | Some a => Some a
+    | None => o'
+    end
+  with
+  | Some a => a
+  | None => d
+  end =
+  match o with
+  | Some a => a
+  | None =>
+      match o' with
+      | Some a => a
+      | None => d
+      end
+  end.
+  Proof. intros. now destruct o, o'. Qed.
+
+  Ltac solve_log_irrelevance'' :=
+    repeat match goal with
+    | H: ?A = ?A |- _ => clear H
+    | H: ∀ _ _ _ _ _ _ _ _ _ _ _ _,
+      interp_action _ _ _ (log_app _ _) _ _ = Some _ ->
+      interp_action _ _ _ _ _ _ = Some _,
+      H1: interp_action _ _ _ (log_app _ _ ) _ _ = Some _ |- _=>
+      pose_once (H _ _ _ _ _ _ _ _ _ _ _ _ H1)
+    | H: interp_action ?env ?sig ?Gam ?slog ?alog ?a = Some _ |-
+      context[interp_action ?env ?sig ?Gam ?slog ?alog ?a] =>
+      rewrite H
+    | H: log_app _ ?l = log_app _ (log_app _ ?l) |- _ =>
+      rewrite log_app_assoc in H;
+      apply log_app_inv_tail in H
+    | H: (if ?cond then Some _ else None) = Some _ |- _ =>
+    destruct (cond) eqn:?Hc; inversion H
+    | _ => progress simple_interp_some
+    | _ => progress cbn
+    | H: context[may_read] |- _ => unfold may_read in H
+    | |- context[may_read] => unfold may_read
+    | H: match ?p with | P0 => _ | P1 => _ end = _ |- _ => destruct p
+    | H: _ && _ = true |- _ => apply andb_prop in H; destruct H
+    | H: _ || _ = false |- _ => rewrite orb_false_iff in H; destruct H
+    | H: negb _ = true |- _ => rewrite negb_true_iff in H
+    | H: context[log_existsb (log_app _ _) _ _] |- _ => rewrite log_existsb_app in H
+    | H: ?A = false |- context[?A] => rewrite H
+    end;
+    try solve [repeat match goal with
+    | |- and _ _ => split
+    | |- log_app (log_app _ _) _ = log_app _ (log_app _ _) => apply eq_sym, log_app_assoc
+    | |- _ => solve [assumption + reflexivity + discriminate]
+    end].
+
+  Fixpoint interp_sched_log_irrelevance sig tau (a : action' R Sigma (sig := sig) (tau := tau)): ∀ (env : REnv.(env_t) R) sigma Γ Γ' slog slog' alog alog_out r,
+    interp_action env sigma Γ (log_app slog slog') alog a = Some (alog_out, r, Γ') ->
+    interp_action (commit_update env slog') sigma Γ slog alog a = Some (alog_out, r, Γ').
+  Proof.
+    destruct a; cbn; intros; try solve [solve_log_irrelevance''].
+    - solve_log_irrelevance''.
+      destruct (Bits.single t0);
+      solve_log_irrelevance''.
+    - solve_log_irrelevance''.
+      +
+        rewrite ?log_existsb_app.
+        solve_log_irrelevance''.
+        f_equal.
+        f_equal.
+        f_equal.
+        (* unfold commit_update. *)
+        rewrite getenv_commit_update.
+        now rewrite latest_write_None.
+      + rewrite ?log_existsb_app.
+        solve_log_irrelevance''.
+        f_equal.
+        f_equal.
+        f_equal.
+
+        rewrite getenv_commit_update.
+
+        rewrite log_app_assoc.
+        rewrite (latest_write0_app _ slog') at 1.
+        rewrite latest_write_latest_write0 by easy.
+        apply eq_sym, option_match_eq.
+    - solve_log_irrelevance''.
+      unfold may_write in *.
+      solve_log_irrelevance'';
+      rewrite ?log_existsb_app;
+      solve_log_irrelevance''.
+    - solve_log_irrelevance''.
+  Admitted.
+
+  Fixpoint interp_sched_log_irrelevance'' sig tau (a : action' R Sigma (sig := sig) (tau := tau)): ∀ (env : REnv.(env_t) R) sigma Γ Γ' Γ'' slog slog' alog alog_out alog_out' r r',
+    interp_action env sigma Γ (log_app slog slog') alog a = Some (alog_out, r, Γ') ->
+    interp_action (commit_update env slog') sigma Γ slog alog a = Some (alog_out', r', Γ'') ->
+
+    alog_out = alog_out' /\ r = r' /\ Γ' = Γ''.
+  Proof.
+    destruct a; cbn; intros; try solve [solve_log_irrelevance'].
+    - solve_log_irrelevance'.
+      destruct (Bits.single t0);
+      solve_log_irrelevance'.
+    - solve_log_irrelevance'.
+      repeat split.
+      clear H7 H6 H5 H4 H3 H2.
+      rewrite getenv_commit_update.
+      unfold may_read in Hc0.
+      destruct port.
+      + apply andb_prop in Hc0.
+        destruct Hc0.
+        rewrite negb_true_iff, log_existsb_app, orb_false_iff in H0, H.
+        destruct H, H0.
+        rewrite log_existsb_app, orb_false_iff in H1, H2.
+        destruct H1, H2.
+        now rewrite latest_write_None.
+      + rewrite log_app_assoc.
+        rewrite latest_write0_app.
+
+        rewrite latest_write_latest_write0.
+        apply option_match_eq.
+
+        rewrite negb_true_iff, log_existsb_app, orb_false_iff in Hc0.
+        destruct Hc0.
+        rewrite log_existsb_app, orb_false_iff in H0.
+        destruct H0.
+        auto.
+    - solve_log_irrelevance'.
+      enough (∀ l1 l t4 t0 Γ Γ' Γ'',
+        interp_args env sigma Γ (log_app slog slog') alog args = Some (l1, t4, Γ') ->
+        interp_args (commit_update env slog') sigma Γ slog alog args = Some (l, t0, Γ'') ->
+        l1 = l /\ t4 = t0 /\ Γ' = Γ''
+      ).
+      + specialize (H _ _ _ _ _ _ _ Heq0 Heq).
+        destruct H, H0.
+        subst.
+        solve_log_irrelevance'.
+      + clear Heq0 Heq Heq1 Heq2 fn t4 Γ Γ' Γ'' t0 t1 t5.
+         (* intros. *)
+        induction args.
+        * intros. cbn in H, H0.
+          solve_log_irrelevance'.
+        * intros. cbn in H, H0.
+          solve_log_irrelevance'.
+          specialize (IHargs _ _ _ _ _ _ _ Heq0 Heq).
+          solve_log_irrelevance'.
+  Qed.
+
+  Ltac solve_log_irrelevance''' :=
+    repeat match goal with
+    | H: ∀ _ _ _ _ _ _ _ _ _ _ _,
+      interp_action _ _ _ _ _ _ = Some _ ->
+      ∃ _, _,
+      Hin: interp_action ?env _ _ ?slog ?alog _ = Some _ |-
+      context [interp_action (commit_update ?env (log_app ?alog ?slog))] =>
+      pose_once (H _ _ _ _ _ _ _ _ _ _ _ Hin)
+    | H: interp_action ?env ?sig ?Gam ?slog ?alog ?a = Some _ |-
+      context[interp_action ?env ?sig ?Gam ?slog ?alog ?a] =>
+      rewrite H
+    | H: ∃ _, _ |- _ => destruct H
+    | H: context[let _ := _ in _] |-  _ =>
+      cbv zeta in H
+    | H: log_app _ ?l = log_app _ (log_app _ ?l) |- _ =>
+      rewrite log_app_assoc in H;
+      apply log_app_inv_tail in H
+    | H: (if ?cond then Some _ else None) = Some _ |- _ =>
+    destruct (cond) eqn:?Hc; inversion H
+    | _ => progress simple_interp_some
+    | _ => progress cbn
+    end;
+    try solve [repeat match goal with
+    | |- and _ _ => split
+    | |- log_app (log_app _ _) _ = log_app _ (log_app _ _) => apply eq_sym, log_app_assoc
+    | |- _ => solve [assumption + reflexivity + discriminate]
+    end].
+
+  Fixpoint interp_log_irrelevance'' sig tau (a : action' R Sigma (sig := sig) (tau := tau)) : ∀  (env : REnv.(env_t) R) sigma Γ Γ' slog alog alog_out r,
+    interp_action env sigma Γ slog alog a = Some (alog_out, r, Γ') ->
+    exists alog_out',
+    interp_action (commit_update env (log_app alog slog)) sigma Γ log_empty log_empty a = Some (alog_out', r, Γ') /\
+    alog_out = log_app alog_out' alog.
+  Proof.
+  Admitted.
+    (* destruct a; cbn; intros.
+    - eexists. solve_log_irrelevance.
+    - eexists. rewrite commit_update_empty. now inversion H.
+    - eexists. solve_log_irrelevance.
+      now rewrite commit_update_empty.
+    - solve_log_irrelevance'''.
+      eexists.
+      now split.
+    - solve_log_irrelevance'''.
+      clear H H0 Heq t0.
+      pose proof (interp_log_irrelevance'' _ _ _ _ _ _ _ _ _ _ _ H1).
+      solve_log_irrelevance'''.
+      rewrite H2 in H.
+      assert (interp_action (commit_update env (log_app alog slog)) sigma t log_empty x a2 = Some (x0, r, Γ')).
+  Admitted. *)
+
+  Context {sig: tsig TypedParsing.var_t}.
+  Section idk.
+    Context {tau: type}.
+    Notation action := (action' R Sigma (sig := sig) (tau := tau)).
+
+    Definition assertion := REnv.(env_t) R -> tcontext sig -> Prop.
+
+    Definition aTrue : assertion := fun _ _  => True.
+    Definition aFalse : assertion := fun _ _  => False.
+
+    Definition aImpl (P Q : assertion) : Prop :=
+      forall env Γ, P env Γ -> Q env Γ.
+
+    Definition aIff (P Q : assertion) : Prop :=
+      aImpl P Q /\ aImpl P Q.
+
+    Notation "P '->>' Q" := (aImpl P Q) (at level 80).
+
+    Notation "P '<<->>' Q" := (aIff P Q) (at level 80).
+
+    Definition hoare_triple
+      (P : assertion) (a : action) (Q : tau -> assertion) : Prop :=
+      ∀ env Γ Γ' sigma log r,
+      P env Γ ->
+      interp_action env sigma Γ log_empty log_empty a = Some (log, r, Γ') ->
+      Q r (commit_update env log) Γ'.
+
+    Lemma hoare_logs : ∀ P a Q,
+      hoare_triple P a Q ->
+      ∀ env Γ Γ' sigma slog alog alog' r,
+      P (commit_update env (log_app alog slog)) Γ ->
+      interp_action env sigma Γ slog alog a = Some (alog', r, Γ') ->
+      Q r (commit_update env (log_app alog' slog)) Γ'.
+    Proof.
+      intros P a Q Hht env Γ Γ' sigma slog alog alog' r HP Hin.
+      unfold hoare_triple in Hht.
+      apply interp_log_irrelevance'' in Hin.
+      destruct Hin as [log [Hin  Hlog]].
+      specialize (Hht (commit_update env (log_app alog slog)) Γ Γ' sigma _ _ HP Hin).
+      rewrite commit_update_assoc, log_app_assoc, <- Hlog in Hht.
+      assumption.
+    Qed.
+  End idk.
+
+  Local Ltac specialize_hoare :=
+    match goal with
+    | HP: ?P _ _,
+      HHT: hoare_triple ?P ?a _,
+      Hin: interp_action _ _ _ _ _ ?a = Some _ |- _=>
+      specialize (HHT _ _ _ _ _ _ HP Hin)
+    end.
+
+  (* todo checkout custom assignment notations from sf*)
+  (* todo check level *)
+  Notation "'{{' P '}}' a '{{' Q '}}'" := (hoare_triple P a Q) (at level 10).
+    (* ( P custom assn at level 99, , Q custom assn at level 99) *)
+
+  Notation action tau := (action' R Sigma (sig := sig) (tau := tau)).
+
+  Theorem hoare_post_true tau : ∀ P (a : action tau),
+    (* hoare_triple P a (fun _ => aTrue). *)
+    {{ P }} a {{ fun _ => aTrue }}.
+  Proof. now unfold hoare_triple, aTrue. Qed.
+
+  Theorem hoare_pre_false tau : ∀ Q (a : action tau),
+    {{ aFalse }} a {{ Q }}.
+  Proof. now unfold hoare_triple, aFalse. Qed.
+
+  Theorem hoare_pass : ∀ P,
+    {{ P }} <{ pass }> {{ fun _ => P}}.
+  Proof. intros * ? * HP; inversion 1; subst.
+    rewrite commit_update_empty; assumption. Qed.
+
+  Theorem hoare_seq {tau} : ∀ P Q R c1 (c2 : action tau),
+    {{ Q }} c2 {{ R }} →
+    {{ P }} c1 {{ fun _ => Q }} →
+    {{ P }} <{ `c1`; `c2` }> {{ R }}.
+  Proof.
+    intros * Hc2 Hc1 ? * HP Hinterp.
+    simple_interp_some.
+    specialize_hoare; cbv beta in Hc1.
+    rewrite <- (log_app_empty_r _ l) in Hc1.
+    pose proof (Hl := hoare_logs _ _ _ Hc2  _ _ _ _ _ _ _ _ Hc1 H0).
+    now rewrite <- (log_app_empty_r _ log).
+  Qed.
+
+  Theorem hoare_consequence {tau} : ∀ P P' Q Q' (a : action tau),
+    {{ P' }} a {{ Q' }} ->
+    (forall env Γ, P env Γ -> P' env Γ) ->
+    (forall env Γ ret, Q' ret env Γ -> Q ret env Γ) ->
+    {{ P }} a {{ Q }}.
+  Proof. unfold hoare_triple. eauto. Qed.
+
+  Theorem hoare_read `{FiniteType reg_t} : ∀ P port reg,
+    {{ P }} (Read port reg) {{ fun ret env Γ => ret = getenv _ env reg /\ P env Γ }}.
+  Proof.
+    intros * ? * HP Hint.
+    cbn in Hint.
+    rewrite may_read_empty in Hint.
+    inversion Hint.
+
+    solve_log_irrelevance.
+    repeat match goal with
+    | H: ?A = ?A |- _ => clear H
+    end.
+    split;
+      [destruct port;
+        [| rewrite (log_app_empty_r _ _), latest_write0_empty]|];
+      now rewrite commit_read, commit_update_empty.
+  Qed.
+
+  Theorem hoare_if_true tau : ∀ P Q R (c : action (bits_t 1)) (tr fl : action tau),
+    {{ P }} c {{ fun ret env Γ => ret = Ob~1 /\ R env Γ }} ->
+    {{ R }} tr {{ Q }} ->
+    {{ P }} <{if `c` then `tr` else `fl`}> {{ Q }}.
+  Proof.
+    intros ** ? * HP Hin.
+    solve_log_irrelevance.
+    unfold hoare_triple in H.
+    specialize (H _ _ _ _ _ _ HP Heq).
+    solve_log_irrelevance.
+    cbn in H2.
+    rewrite <- (log_app_empty_r _ l) in H1.
+    pose proof (hoare_logs _ _ _ H0 _ _ _ _ _ _ _ _ H1 H2).
+    now rewrite <- (log_app_empty_r _ log).
+  Qed.
+
+  Theorem hoare_if_false tau : ∀ P Q R (c : action (bits_t 1)) (tr fl : action tau),
+    {{ P }} c {{ fun ret env Γ => ret = Ob~0 /\ R env Γ }} ->
+    {{ R }} fl {{ Q }} ->
+    {{ P }} <{if `c` then `tr` else `fl`}> {{ Q }}.
+    intros ** ? * HP Hin.
+    solve_log_irrelevance.
+    unfold hoare_triple in H.
+    specialize (H _ _ _ _ _ _ HP Heq).
+    solve_log_irrelevance.
+    cbn in H2.
+    rewrite <- (log_app_empty_r _ l) in H1.
+    pose proof (hoare_logs _ _ _ H0 _ _ _ _ _ _ _ _ H1 H2).
+    now rewrite <- (log_app_empty_r _ log).
+  Qed.
+
+  (* Reserved Notation "'{{' P '}}' a '{{' Q '}}'" (at level 40). *)
+  Inductive HoareTriple : forall {tau : type}, assertion -> action sig tau -> (tau -> assertion) -> Prop :=
+  | HTSeq : ∀ tau P Q R a1 a2,
+  (* TODO maybe swap preconditions *)
+    HoareTriple P a1 Q ->
+    (forall r, HoareTriple (Q r) a2 R) ->
+    @HoareTriple tau P (Seq a1 a2) R
+  | HTFail : ∀ tau P Q,
+    HoareTriple P (Fail tau) Q
+  | HTIf : ∀ tau P Q R cond tr fl,
+    (@HoareTriple (bits_t 1) P cond (fun ret e Γ sl al => ret = Ob~1 /\ Q e Γ sl al) /\ @HoareTriple tau Q tr R) \/
+    (@HoareTriple (bits_t 1) P cond (fun ret e Γ sl al => ret = Ob~0 /\ Q e Γ sl al) /\ @HoareTriple tau Q fl R) ->
+    HoareTriple P (If cond tr fl) R
+  | HTConst : ∀ tau cst P,
+    @HoareTriple tau P (Const cst) (fun r _ _ _ _ => r = cst)
+  | HTVar : ∀ tau nm m P,
+    @HoareTriple tau P (Var m (k := nm)) (fun r _ Γ _ _ => r = cassoc m Γ)
+  (* strengthen precondition + weaken postcondition *)
+  | HTConsequence : forall tau P Q P' Q' c,
+    @HoareTriple tau P c Q ->
+    (forall e G sl al, P' e G sl al -> P e G sl al) ->
+    (forall r e G sl al, Q r e G sl al -> Q' r e G sl al) ->
+    @HoareTriple tau P' c Q'
+  | HTBinop : forall fn a1 a2 P Q R v1 v2,
+    HoareTriple P a1 (fun r e Γ sl al => r = v1 /\ Q e Γ sl al) ->
+    HoareTriple Q a2 (fun r e Γ sl al => r = v2 /\ R e Γ sl al) ->
+    HoareTriple P (Binop fn a1 a2) (fun r e Γ sl al => r = ((PrimSpecs.sigma2 fn) v1 v2) /\ R e Γ sl al).
+  (* where "{{ P }} a {{ Q }}" := (HoareTriple (fun env Γ sl al => P) a (fun ret env Γ sl al => Q)). *)
+
+  Fixpoint hoare_triple_interp_action {tau} P (a : action sig tau) Q (ht : HoareTriple P a Q) {struct ht}:
+    ∀ env Γ Γ' sigma r slog alog alog',
+    P env Γ alog slog ->
+    interp_action env sigma Γ slog alog a = Some (alog', r, Γ') ->
+    Q r env Γ' alog' slog.
+  Proof.
+    induction ht.
     - intros.
       simpl in H2.
       destruct (interp_action env sigma Γ slog alog a1) eqn:Heq; inversion H2.
       do 2 destruct p. clear H2.
-      specialize (IHHoareTriple1 _ _ _ _ _ _ _ _ H1 Heq).
-      specialize (IHHoareTriple2 _ _ _ _ _ _ _ _ IHHoareTriple1 H4).
+      specialize (IHht _ _ _ _ _ _ _ _ H1 Heq).
+      specialize (H0 _ _ _ _ _ _ _ _ _ IHht H4).
       assumption.
+    - intros.
+      simpl in H0. inversion H0.
+    - intros.
+      repeat match goal with
+      | H: interp_action _ _ _ _ _ ?a = Some _ |- _ => head_constructor a; simpl in H
+      | H: opt_bind ?a _ = Some _ |- _ => destruct a eqn:?Heq; inversion H; clear H
+      | H: prod _ _ |- _ => destruct H
+      end.
+      destruct H.
+      + destruct H.
+        pose proof (hoare_triple_interp_action _ _ _ _ H _ _ _ _ _ _ _ _ H0 Heq).
+        simpl in H2.
+        destruct H2.
+        rewrite H2 in H3.
+        simpl in H3.
+        pose proof (hoare_triple_interp_action _ _ _ _ H1 _ _ _ _ _ _ _ _ H4 H3).
+        assumption.
+      + destruct H.
+        pose proof (hoare_triple_interp_action _ _ _ _ H _ _ _ _ _ _ _ _ H0 Heq).
+        simpl in H2.
+        destruct H2.
+        rewrite H2 in H3.
+        simpl in H3.
+        pose proof (hoare_triple_interp_action _ _ _ _ H1 _ _ _ _ _ _ _ _ H4 H3).
+        assumption.
+    - intros.
+      simpl in H0. inversion H0. reflexivity.
+    - intros.
+      simpl in H0.
+      inversion H0. reflexivity.
+    - intros.
+      clear hoare_triple_interp_action.
+      eauto.
+    - intros.
+      repeat match goal with
+      | H: interp_action _ _ _ _ _ ?a = Some _ |- _ => head_constructor a; simpl in H
+      | H: opt_bind ?a _ = Some _ |- _ => destruct a eqn:?Heq; inversion H; clear H
+      | H: prod _ _ |- _ => destruct H
+      end.
+      specialize (IHht1 _ _ _ _ _ _ _ _ H Heq).
+      destruct IHht1. subst.
+      specialize (IHht2 _ _ _ _ _ _ _ _ H2 Heq0).
+      destruct IHht2. subst.
+      inversion H1.
+      split. reflexivity. subst. auto.
   Qed.
+
+  Definition HoareTriple2 {tau} :
+    action sig tau ->
+    assertion -> (tau -> assertion) -> Prop :=
+    fun a P Q => HoareTriple P a Q.
+End Hoare.
+
+Require Import Koika.Frontend.
+Require Import Koika.TypedParsing.
+
+Inductive empty_reg_t :=.
+Definition empty_R (r : empty_reg_t) : type := match r with end.
+
+Definition min : function empty_R empty_Sigma := <{
+fun min (a : bits_t 5) (b : bits_t 5) : bits_t 5 =>
+  if (a < b)
+    then a
+    else b
+}>.
+
+Definition convert_ctx {K sig} : @TypedSemantics.tcontext K sig ->
+  context (fun k_tau : K * type => snd k_tau) sig.
+  exact id.
+Defined.
+
+Notation "ctx .[ f ]" := (@cassoc _ _ _ (f,_) _ (convert_ctx ctx)).
+Set Typeclasses Debug.
+
+
+Notation "{ P } a { Q }" := (HoareTriple P a Q) (only printing).
+(* Notation "{ P } a { Q }" := (HoareTriple (fun _ _ _ _ => P) a Q) (only printing). *)
+
+Lemma min_correct m n env:
+  HoareTriple2 (REnv := env)
+  min.(int_body)
+  (fun _ Γ _ _ => Γ.["a"] = Bits.of_nat 5 m /\ Γ.["b"] = Bits.of_nat 5 n)
+  (fun r _ _ _ _ => r = Bits.of_nat 5 m ).
+Proof.
+  unfold HoareTriple2.
+  unfold min, int_body.
+  unfold TypedParsing.refine_sig_tau.
+  eapply HTIf.
+
+  destruct (m <? n)%nat eqn:Hc.
+  - left.
+    split.
+    eapply HTConsequence.
+    change (bits_t 1) with (retSig (PrimSignatures.Sigma2 (Bits2 (Compare false cLt 5)))).
+    eapply HTBinop.
+    eapply HTVar.
+
+    2: {
+      eapply HTConsequence.
+      - apply HTVar.
+      - intros ? ? ? ?; exact (id).
+      - cbv beta. intros. subst. reflexivity. simpl.
+    2:
+  - right.
+    split.
