coq/TypedSyntax.v
@@ -54,6 +54,81 @@ Section Syntax.
   | APos {sig tau} (pos: pos_t) (a: action sig tau)
     : action sig tau.
 
+  Fixpoint ctx_Forall {K} {V: K -> Type} (P: forall (k: K), V k -> Prop) {sig} (ctx: context V sig) :=
+    match ctx with
+    | CtxEmpty => True
+    | CtxCons k v ctx => P k v /\ ctx_Forall P ctx
+    end.
+
+  Lemma action_ind_complete :
+    forall P : forall (sig : tsig var_t) (tau : type), action sig tau -> Prop,
+
+    (forall (sig : tsig var_t) (tau : type),
+      P sig tau (Fail tau)) ->
+    (forall (sig : list (var_t * type)) (k : var_t) (tau : type) (m : member (k, tau) sig),
+      P sig tau (Var m)) ->
+    (forall (sig : tsig var_t) (tau : type) (cst : tau),
+      P sig tau (Const cst)) ->
+    (forall (sig : list (var_t * type)) (k : var_t) (tau : type) (m : member (k, tau) sig) (ex : action sig tau),
+      P sig tau ex ->
+      P sig unit_t (Assign m ex)) ->
+    (forall (sig : tsig var_t) (tau : type) (r1 : action sig unit_t) (r2 : action sig tau),
+      P sig unit_t r1 ->
+      P sig tau r2 ->
+      P sig tau (Seq r1 r2)) ->
+    (forall (sig : tsig var_t) (tau tau' : type) (var : var_t) (ex : action sig tau) (body : action ((var, tau) :: sig) tau'),
+      P sig tau ex ->
+      P ((var, tau) :: sig) tau' body ->
+      P sig tau' (Bind var ex body)) ->
+    (forall (sig : tsig var_t) (tau : type) (cond : action sig (bits_t 1)) (tbranch : action sig tau) (fbranch : action sig tau),
+      P sig (bits_t 1) cond ->
+      P sig tau tbranch ->
+      P sig tau fbranch ->
+      P sig tau (If cond tbranch fbranch)) ->
+    (forall (sig : tsig var_t) (port : Port) (idx : reg_t),
+      P sig (R idx) (Read port idx)) ->
+    (forall (sig : tsig var_t) (port : Port) (idx : reg_t) (value : action sig (R idx)),
+      P sig (R idx) value -> P sig unit_t (Write port idx value)) ->
+    (forall (sig : tsig var_t) (fn : fn1) (arg1 : action sig (arg1Sig (Sigma1 fn))),
+      P sig (arg1Sig (Sigma1 fn)) arg1 ->
+      P sig (retSig (Sigma1 fn)) (Unop fn arg1)) ->
+    (forall (sig : tsig var_t) (fn : fn2) (arg1 : action sig (arg1Sig (Sigma2 fn))) (arg2 : action sig (arg2Sig (Sigma2 fn))),
+      P sig (arg1Sig (Sigma2 fn)) arg1 ->
+      P sig (arg2Sig (Sigma2 fn)) arg2 ->
+      P sig (retSig (Sigma2 fn)) (Binop fn arg1 arg2)) ->
+    (forall (sig : tsig var_t) (fn : ext_fn_t) (arg : action sig (arg1Sig (Sigma fn))),
+      P sig (arg1Sig (Sigma fn)) arg ->
+      P sig (retSig (Sigma fn)) (ExternalCall fn arg)) ->
+    (forall (sig : tsig var_t) (tau : type) (argspec : tsig var_t) (fn : InternalFunction' fn_name_t (action argspec tau)) (args : context (fun k_tau : var_t * type => action sig (snd k_tau)) argspec),
+      P argspec tau fn.(int_body) ->
+      ctx_Forall (fun k_tau => P sig (snd k_tau)) args ->
+      P sig tau (InternalCall fn args)) ->
+    (forall (sig : tsig var_t) (tau : type) (pos : pos_t) (a : action sig tau),
+      P sig tau a -> P sig tau (APos pos a)) ->
+    forall (sig : tsig var_t) (tau : type) (a : action sig tau), P sig tau a.
+  Proof.
+    intros P H1 H2 H3 H4 H5 H6 H7 H8 H9 H10 H11 H12 H13 H14.
+    fix IH 3.
+    destruct a.
+    - apply H1.
+    - apply H2.
+    - apply H3.
+    - apply H4. auto.
+    - apply H5; auto.
+    - apply H6; auto.
+    - apply H7; auto.
+    - apply H8.
+    - apply H9. auto.
+    - apply H10. auto.
+    - apply H11; auto.
+    - apply H12. auto.
+    - apply H13. auto. clear fn.
+      induction args.
+      + cbn. auto.
+      + split. auto. assumption.
+    - apply H14. auto.
+  Qed.
+
   Definition rule := action nil unit_t.
 End Syntax.
 
