coq/SeperationLogic.v
@@ -1,0 +1,185 @@
+(* Implementing hoare logic for koika's evaluation *)
+Require Import Unicode.Utf8.
+
+Require Import Koika.TypedSyntax.
+Require Import Koika.TypedSemantics.
+
+Inductive test_reg_t :=
+  one | two | three | four.
+(*
+Inductive type_list {K}: list K -> Type :=
+| TLNil: type_list []
+| TLCons {l'} (k: K) (ctx: type_list l'): type_list (k :: l').
+
+Require Import Coq.Program.Equality. *)
+
+(* The only element that exists of a type_list *)
+(* Fixpoint finite_element_type_list {K} (l : list K) : type_list l :=
+  match l with
+  | nil => TLNil
+  | cons k l' => TLCons k (finite_element_type_list l')
+  end. *)
+
+
+Definition R (r : test_reg_t) : type := bits_t 4.
+Definition env := ContextEnv.(create) R.
+
+Search (Type -> Type -> Type).
+
+(* This type carries a list on the type level and every element of this type
+  identifies an element of this list *)
+Inductive type_list {K}: list K -> Type :=
+  (* first element of the list *)
+  | TLHead: forall k l, type_list (k :: l)
+  (* later element of the list *)
+  | TLTail: forall k l, type_list l -> type_list (k :: l).
+
+Fixpoint type_list_ft_idx {K} {l : list K} (tl : type_list l) :=
+  match tl with
+  | TLHead _ _ => 0
+  | TLTail _ _ tl' => S (type_list_ft_idx tl')
+  end.
+
+Fixpoint type_list_ft_elem {K} (l : list K) : list (type_list l) :=
+  match l with
+  | [] => []
+  | k :: l' => TLHead _ _ :: map (TLTail _ _) (type_list_ft_elem l')
+  end.
+
+Lemma type_list_ft_seq {K} {l : list K} :
+  map type_list_ft_idx (type_list_ft_elem l) = seq 0 (List.length l).
+Proof.
+  induction l as [| ? ? IH]. reflexivity.
+  cbn; f_equal. rewrite map_map. cbn. rewrite <- map_map, IH.
+  apply seq_shift.
+Qed.
+
+#[refine] Instance type_list_ft {K} {l : list K} : FiniteType (type_list l) := {
+  finite_index := type_list_ft_idx;
+  finite_elements := (type_list_ft_elem l);
+}.
+  - intro a; induction a; try reflexivity.
+    simpl in *. apply map_nth_error. assumption.
+  - rewrite type_list_ft_seq.
+    apply seq_NoDup.
+Defined.
+
+Definition R_part1 (r : type_list [one; two]) : type := bits_t 4.
+Definition R_part2 (r : type_list [two; three]) : type := bits_t 8.
+
+Definition env1 := ContextEnv.(create) R_part1.
+Definition env2 := ContextEnv.(create) R_part2.
+
+Require Import Koika.Frontend.
+
+Definition some_action : UInternalFunction test_reg_t empty_ext_fn_t :=
+{{
+fun some_action (a : bits_t 0) : unit_t =>
+  read0(one);
+  pass
+}}.
+
+Class ElemOfTL {K} (k : K) (l : list K):= el_of_tl : type_list l.
+
+Instance ElemOfTLHead {K} {k : K} {l'} : ElemOfTL k (cons k l') := TLHead k l'.
+Instance ElemOfTLTail {K} {k k': K} {l'} {eotl : ElemOfTL k l'} : ElemOfTL k (cons k' l') := TLTail k' l' eotl.
+
+
+Arguments el_of_tl {K} k {l} {ElemOfTL} : assert.
+(* Instance tl_head : type_list [] *)
+
+Definition test : type_list [one; two] := el_of_tl two.
+
+Compute test.
+
+Declare Scope type_list_scope.
+Notation "'[[' ']]'" := (type_list []) : type_list_scope.
+Notation "'[[' a ';' .. ';' b ']]'" := (type_list (cons a .. (cons b nil) ..)) : type_list_scope.
+
+Open Scope type_list_scope.
+
+(* Notation "'>' reg" := (el_of_tl reg) (in custom koika at level 0, reg constr). *)
+
+Definition some_action2 : UInternalFunction [[ ]] empty_ext_fn_t :=
+{{
+fun some_action (a : bits_t 0) : unit_t =>
+  pass
+}}.
+
+Definition some_action : action
+
+
+Section SepLog.
+
+  Definition hprop {reg_t} {R : reg_t -> type} {REnv : Env reg_t}
+    := REnv.(env_t) R -> Prop.
+  (* Implication *)
+  Definition himp {reg_t} {R : reg_t -> type} {REnv : Env reg_t}
+    (p q : @hprop reg_t R REnv) := forall h, p h -> q h.
+  (* Equivalence *)
+  Definition heq {reg_t} {R : reg_t -> type} {REnv : Env reg_t}
+    (p q : @hprop reg_t R REnv) := forall h, p h <-> q h.
+  (* Lifting a pure proposition: it must hold, and the heap must be empty. *)
+  Inductive empty_reg_t :=.
+  Definition empty_R (r : empty_reg_t) : type := match r with end.
+  Definition empty_r (r : empty_reg_t) : type_denote (empty_R r) := match r with end.
+  Definition lift {REnv : Env _} (P : Prop) : @hprop empty_reg_t empty_R REnv :=
+    fun h => P /\ h = (REnv.(create) (fun r => match r with end)).
+
+
+End SepLog.
+
+Section SeperationLogic.
+
+  Context {pos_t var_t fn_name_t reg_t ext_fn_t: Type}.
+  Context {R: reg_t -> type}.
+  Context {Sigma: ext_fn_t -> ExternalSignature}.
+
+  Notation action := (action pos_t var_t fn_name_t R Sigma).
+
+  (* Register environment a Map-Type from register names to their values *)
+  Context {REnv: Env reg_t}.
+  Context {sig: tsig var_t}.
+
+
+
+
+  Definition assertion := tcontext sig -> REnv.(env_t) R -> Prop.
+
+  Inductive HoareTriple {tau: type} : assertion -> action sig tau -> (tau -> assertion) -> Prop :=
+  | HTSeq : ∀ P Q R a1 a2,
+    HoareTriple P a1 Q -> (forall r, HoareTriple (Q r) a2 R) ->
+    HoareTriple P (Seq a1 a2) R
+  | HTFail :
+    HoareTriple (fun _ _ => False) (Fail tau) (fun _ _ _ => False).
+
+  Declare Scope log_scope.
+  Notation "[]" := log_empty : log_scope.
+  Bind Scope log_scope with Log.
+
+  Definition interp_action_update_env {tau} env sigma Gamma slog alog (act : action sig tau) :=
+    option_map (fun '(l, r, Gamma') => (commit_update env l, r, Gamma')) (interp_action (REnv := REnv) env sigma Gamma slog alog act).
+
+  (* Definition interp_weaken_log :
+    interp_action env sigma Gamma slog alog a = Some (l, r, Gamma') -,> *)
+
+  Theorem hoare_triple_interp_action {tau} : ∀ P (a : action sig tau) Q,
+    HoareTriple P a Q ->
+    ∀ env Γ Γ' sigma r slog alog alog',
+    P Γ (commit_update env (log_app alog slog)) ->
+    interp_action env sigma Γ slog alog a = Some (alog', r, Γ') ->
+    Q r Γ' (commit_update env (log_app alog' slog)).
+  Proof.
+    induction 1.
+    - intros.
+      simpl in H2.
+      destruct (interp_action env sigma Γ slog alog a1) eqn:Heq; inversion H2.
+      do 2 destruct p. clear H2.
+      specialize (IHHoareTriple1 _ _ _ _ _ _ _ _ H1 Heq).
+      specialize (fun log => IHHoareTriple2 (commit_update env l) log t).
+
+
+
+      specialize (IHHoareTriple2 _ _ _ _ _ _ _ _ IHHoareTriple1 H4).
+      assumption.
+  Qed.
